Align with lecture and add explanations

Policies/Noninterference/Automata.thy
@@ -4,20 +4,45 @@ theory Automata
 imports Main
 begin
 
+text \<open>We consider automata defined by a type @{text "'state"} (corresponding to a non-empty set)
+of states, a type @{text "'act"} of actions, a type @{text "'out"} of outputs, a starting state
+@{text s0}, a step function @{text step}, and an output function @{text out}.\footnote{The
+Isabelle command @{text locale} opens a new context where we can fix variables and/or define
+assumptions. We can use these variables and assumptions inside the context, and we can reuse
+and extend the context later by referring to its name (in this case @{text "Automaton"}).
+We can also @{emph \<open>instantiate\<close>} a context (using the command @{text \<open>interpretation\<close>},
+or @{emph \<open>sublocale\<close>} if we are inside another context): We then have to prove that the
+assumptions hold, and afterwards, we are allowed to use the definitions and theorems from
+inside the context.}\<close>
+
 locale Automaton =
   fixes s0 :: "'state"
     and step :: "'state \<Rightarrow> 'act \<Rightarrow> 'state"
     and out :: "'state \<Rightarrow> 'act \<Rightarrow> 'out"
 begin
 
-primrec run :: "'state \<Rightarrow> 'act list \<Rightarrow> 'state" where
+text \<open>We define @{text "run s \<alpha>"} so that it returns the state we reach when performing the
+action sequence @{text \<alpha>}, beginning in the state @{text s}.\<close>
+
+text \<open>The function @{text run} is defined recursively. In Isabelle, the empty list is denoted
+as @{text "[]"}, the addition of an @{emph \<open>element\<close>} @{text a} at the beginning of a list
+@{text \<alpha>} is denoted as @{text "a # \<alpha>"}, and the concatenation of two @{emph \<open>lists\<close>}
+@{text \<alpha>} and @{text \<beta>} is denoted as @{text "\<alpha> @ \<beta>"}.\<close>
+
+fun run :: "'state \<Rightarrow> 'act list \<Rightarrow> 'state" where
   "run s [] = s"
 | "run s (a # \<alpha>) = run (step s a) \<alpha>"
 
-lemma "\<forall>s. (run s \<alpha> = t \<and> run t \<beta> = u) \<longrightarrow> run s (\<alpha> @ \<beta>) = u"
-by (induction \<alpha>) auto
+text \<open>After writing down definitions, Isabelle allows us to prove properties of them. For example,
+we can (almost\footnote{We tell Isabelle to perform induction over @{text \<alpha>}. Moreover, we
+tell Isabelle to generalize the induction hypothesis to arbitrary states @{text s}, because
+we need to apply the induction hypothesis not for the original @{text s}, but for the successor
+state reached after performing the first action of the trace.}) automatically prove that we can
+concatenate two traces of actions, if the first trace ends in the starting state of the second.\<close>
+
+lemma "\<lbrakk>run s \<alpha> = t \<and> run t \<beta> = u\<rbrakk> \<Longrightarrow> run s (\<alpha> @ \<beta>) = u"
+by (induction \<alpha> arbitrary: s) auto
 
 end
 
 end
-
