Policies/Reference_Monitor/Simple_Lang.thy
@@ -4,34 +4,58 @@ theory Simple_Lang
 imports Main
 begin
 
+text \<open>In this example we will use the above theorem to prove the security of a very simplistic
+programming language incorporating a reference monitor.\<close>
+
 subsubsection {* Language *}
 
-type_synonym 'var state = "'var \<Rightarrow> integer"
+text \<open>As actions, we only consider assignments of the form @{text "n :=\<^bsub>d\<^esub> \<tau>"}, where @{text n}
+is a variable name, @{text d} is a domain, and @{text \<tau>} is an expression. We only consider basic
+expressions that are built using variable references and addition:\<close>
 
 datatype 'var expr =
   Var 'var
 | Plus "'var expr" "'var expr"
 
-primrec eval :: "'var state \<Rightarrow> 'var expr \<Rightarrow> integer" where
-  "eval s (Var v) = s v"
-| "eval s (Plus e1 e2) = eval s e1 + eval s e2"
+text \<open>For example, @{text "Plus (Plus (Var a) (Var b)) (Var c)"} is an expression and denotes the
+addition of the variables @{text a}, @{text b}, and @{text c}.
 
-primrec FV :: "'var expr \<Rightarrow> 'var set" where
-  "FV (Var v) = {v}"
-| "FV (Plus e1 e2) = FV e1 \<union> FV e2"
+The state of the automaton is simply a mapping from variable names to integers.\<close>
+
+type_synonym 'var state = "'var \<Rightarrow> integer"
+
+text \<open>The function @{text \<E>} evaluates an expression in a given state.\<close>
+
+fun \<E> :: "'var expr \<Rightarrow> 'var state \<Rightarrow> integer" where
+  "\<E> (Var v) s = s v"
+| "\<E> (Plus e1 e2) s = \<E> e1 s + \<E> e2 s"
+
+text \<open>The function @{text Vars} returns the set of variables appearing in an expression.\<close>
+
+primrec Vars :: "'var expr \<Rightarrow> 'var set" where
+  "Vars (Var v) = {v}"
+| "Vars (Plus e1 e2) = Vars e1 \<union> Vars e2"
+
+text \<open>Actions are assignments of expressions to variables, annotated with a domain.\<close>
 
 datatype ('var, 'dom) cmd =
   Assign 'var (dom: 'dom) "'var expr" ("_ :=\<^bsub>_\<^esub> _")
 
-lemma "dom (Assign v d e) = d"
+lemma "dom (v :=\<^bsub>d\<^esub> e) = d"
 by auto
 
-primrec execute :: "'var state \<Rightarrow> ('var, 'dom) cmd \<Rightarrow> 'var state" where
-  "execute s (Assign v d e) = s(v := eval s e)"
+text \<open>The effect of an assignment @{text "v :=\<^bsub>d\<^esub> e"} in a state @{text s} is that the value of
+@{text v} is updated to the evaluation of @{text "e"} in @{text s}.\<close>
+
+fun execute :: "'var state \<Rightarrow> ('var, 'dom) cmd \<Rightarrow> 'var state" where
+  "execute s (v :=\<^bsub>d\<^esub> e) = s(v := \<E> e s)"
+
+text \<open>The following coincidence lemma will be useful: If two states coincide on the variables
+appearing in an expression, then the result of evaluating the expression in both states is equal.\<close>
 
 lemma coincidence:
-  assumes "\<forall>v \<in> FV e. s v = t v"
-  shows "eval s e = eval t e"
+  assumes "\<forall>v \<in> Vars e. s v = t v"
+  shows "\<E> e s = \<E> e t"
 using assms
 by (induction e) auto
 
