Policies/Reference_Monitor/Simple_RM.thy
@@ -4,6 +4,9 @@ theory Simple_RM
 imports Reference_Monitor Simple_Lang
 begin
 
+text \<open>We now define the implementation of a reference monitor for our simple programming language
+(and a given flow policy).\<close>
+
 locale Simple_RM =
   fixes s0 :: "'var state"
     and observe :: "'dom \<Rightarrow> 'var set"
@@ -15,17 +18,23 @@ locale Simple_RM =
       and alter_observe_FP: "n \<in> alter u \<Longrightarrow> n \<in> observe v \<Longrightarrow> (u, v) \<in> FP"
 begin
 
-primrec check :: "('var, 'dom) cmd \<Rightarrow> bool" where
-  "check (v :=\<^bsub>d\<^esub> e) = (v \<in> alter d \<and> FV e \<subseteq> observe d)"
+text \<open>The @{text check} function returns true for an assignment @{text "v :=\<^bsub>d\<^esub> e"} if @{text v}
+is writable by @{text d} and the variables in @{text e} are readable for @{text d}.\<close>
 
-primrec step :: "'var state \<Rightarrow> ('var, 'dom) cmd \<Rightarrow> 'var state" where
+fun check :: "('var, 'dom) cmd \<Rightarrow> bool" where
+  "check (v :=\<^bsub>d\<^esub> e) = (v \<in> alter d \<and> Vars e \<subseteq> observe d)"
+
+text \<open>If the check is successful, the state is updated and the evaluation of the expressions is
+given as output; otherwise, the state remains unchanged, and 0 is given as output.\<close>
+
+fun step :: "'var state \<Rightarrow> ('var, 'dom) cmd \<Rightarrow> 'var state" where
   "step s (v :=\<^bsub>d\<^esub> e) = (if check (v :=\<^bsub>d\<^esub> e)
                          then execute s (v :=\<^bsub>d\<^esub> e)
                          else s)"
 
-primrec out :: "'var state \<Rightarrow> ('var, 'dom) cmd \<Rightarrow> integer" where
+fun out :: "'var state \<Rightarrow> ('var, 'dom) cmd \<Rightarrow> integer" where
   "out s (v :=\<^bsub>d\<^esub> e) = (if check (v :=\<^bsub>d\<^esub> e)
-                        then eval s e
+                        then \<E> e s
                         else 0)"
 
 definition contents :: "'var state \<Rightarrow> 'var \<Rightarrow> integer" where
@@ -33,32 +42,42 @@ definition contents :: "'var state \<Rightarrow> 'var \<Rightarrow> integer" whe
 
 sublocale Automaton s0 step out .
 
-sublocale Structured_State s0 step out contents observe alter .
+text \<open>We currently assume that the consistency conditions for the implementation of the flow policy
+hold (we will have to prove this later for concrete instantiations).\<close>
+
+sublocale FP_Implementation s0 step out contents FP dom observe alter
+using refl_FP trans_FP FP_observe alter_observe_FP
+by unfold_locales
 
 notation view'' ("_ \<sim>\<^bsub>_\<^esub> _")
 
-sublocale NI s0 step out FP dom
-using refl_FP trans_FP 
-by (unfold_locales)
+text \<open>We can, however, already prove generally that the reference monitor assumptions hold.
+
+As a helper lemma, we prove that expressions used in assignments allowed for
+@{text d} are evaluated to the same value in states equivalent for @{text d}.\<close>
 
 lemma view_coincidence:
   assumes "s \<sim>\<^bsub>d\<^esub> t"
       and "check (v :=\<^bsub>d\<^esub> e)"
-  shows "eval s e = eval t e"
+  shows "\<E> e s = \<E> e t"
 proof (intro coincidence)
-  from assms(2) have "FV e \<subseteq> observe d" by auto
-  with assms(1) show "\<forall>v \<in> FV e. s v = t v" unfolding view_def by auto
+  from assms(2) have "Vars e \<subseteq> observe d" by auto
+  with assms(1) show "\<forall>v \<in> Vars e. s v = t v" unfolding view_def by auto
 qed
 
-sublocale Reference_Monitor s0 step out contents observe alter FP dom
+text \<open>We then prove the three reference monitor assumptions.\<close>
+
+sublocale Reference_Monitor s0 step out contents FP dom observe alter
 proof
+  -- \<open>RMA1\<close>
   fix s t fix a :: "('var, 'dom) cmd"
   obtain v d e where [simp]: "a = (v :=\<^bsub>d\<^esub> e)" by (cases a)
   assume "s \<sim>\<^bsub>dom a\<^esub> t"
   then show "out s a = out t a"
   proof (cases "check a")
     case True
-      then have "eval s e = eval t e" using `s \<sim>\<^bsub>dom a\<^esub> t` by (intro view_coincidence) auto
+      then have "\<E> e s = \<E> e t" using `s \<sim>\<^bsub>dom a\<^esub> t`
+        by (intro view_coincidence) auto
       then show "out s a = out t a" using True by auto
   next
     case False
@@ -66,34 +85,27 @@ proof
       then show "out s a = out t a" by auto
   qed
 next
+  -- \<open>RMA2\<close>
   fix s t n fix a :: "('var, 'dom) cmd"
   obtain v d e where [simp]: "a = (v :=\<^bsub>d\<^esub> e)" by (cases a)
   assume "s \<sim>\<^bsub>dom a\<^esub> t"
-     and "contents (step s a) n \<noteq> contents s n \<or> contents (step t a) n \<noteq> contents t n"
+     and "contents (step s a) n \<noteq> contents s n \<or>
+          contents (step t a) n \<noteq> contents t n"
   then have "check a"
-        and "contents (step s a) n = eval s e"
-        and "contents (step t a) n = eval t e"
+        and "contents (step s a) n = \<E> e s"
+        and "contents (step t a) n = \<E> e t"
     by (auto split: split_if_asm)
   then show "contents (step s a) n = contents (step t a) n"
     using `s \<sim>\<^bsub>dom a\<^esub> t`
     by (auto intro: view_coincidence)
 next
+  -- \<open>RMA3\<close>
   fix s n fix a :: "('var, 'dom) cmd"
   obtain v d e where [simp]: "a = (v :=\<^bsub>d\<^esub> e)" by (cases a)
   assume "contents (step s a) n \<noteq> contents s n"
   then have "check a" and "v = n" by (auto split: split_if_asm)
   then show "n \<in> alter (dom a)" by simp
-next
-  fix u v
-  assume "u \<leadsto> v"
-  then show "observe u \<subseteq> observe v" using FP_observe by blast
-next
-  fix n u v
-  assume "n \<in> alter u" and "n \<in> observe v"
-  then show "u \<leadsto> v" using alter_observe_FP by blast
 qed
-
-thm monitor_secure
 
 end
 
