Policies/Noninterference/Noninterference.thy
@@ -4,7 +4,14 @@ theory Noninterference
 imports Automata
 begin
 
+text \<open>We now consider security of such automata in the sense of Goguen and Meseguer's notion
+of @{emph \<open>noninterference\<close>}.\<close>
+
 subsection {* Definition *}
+
+text \<open>For a given automaton, we add a function @{text dom}, which assigns a security domain to each
+action, and a flow policy, which is a reflexive and transitive relation between domains, specifying
+which flows of information are allowed.\<close>
 
 locale NI =
   Automaton s0 step out
@@ -18,21 +25,40 @@ locale NI =
       and "trans FP"
 begin
 
+text \<open>We write @{text "D \<leadsto> D'"} if the flow policy allows a flow from @{text D} to @{text D'}.\<close>
+
 abbreviation flow :: "'dom \<Rightarrow> 'dom \<Rightarrow> bool" ("_ \<leadsto> _")
 where "(D \<leadsto> D') \<equiv> (D, D') \<in> FP"
 
-primrec purge :: "'act list \<Rightarrow> 'dom \<Rightarrow> 'act list" where
+text \<open>We define the @{text purge} function, which removes all actions from a trace @{text \<alpha>} that
+belong to a domain from which no flow is allowed to a given domain @{text D}. In other words,
+we remove actions that should be secret for @{text D}.\<close>
+
+fun purge :: "'act list \<Rightarrow> 'dom \<Rightarrow> 'act list" where
   "purge [] D = []"
 | "purge (a # \<alpha>) D = (if (dom a) \<leadsto> D
                       then a # purge \<alpha> D
                       else purge \<alpha> D)"
 
+text \<open>An automaton is considered secure wrt.\ a noninterference policy if the output of an action
+@{text a} is independent of the execution of secret actions: Purging secret actions from the trace
+that has been executed before does not change the output of @{text a}.\<close>
+
 definition "NI_secure
 \<equiv> \<forall>a \<alpha>. out (run s0 \<alpha>) a = out (run s0 (purge \<alpha> (dom a))) a"
+
+text \<open>This is the @{emph \<open>definition\<close>} of (noninterference) security for automata.
+In the following sections, we focus on techniques for the @{emph \<open>verification\<close>} of security.\<close>
 
 end
 
 subsection {* Verification *}
+
+text \<open>In order to use the unwinding verification technique, we first have to choose a
+@{emph \<open>view partitioning\<close>}, i.e.\ a family of equivalence relations on states, indexed by domain.
+Hence, we have to choose an equivalence relation for each domain. When choosing these relations,
+the intuition is to consider states as equivalent for a domain if they are supposed to be
+indistinguishable for that domain.\<close>
 
 locale View_Partitioning =
   NI s0 step out FP dom
@@ -46,8 +72,13 @@ locale View_Partitioning =
   assumes view_equiv: "\<forall>u. equiv UNIV (view u)"
 begin
 
+text \<open>We write @{text "s \<sim>\<^bsub>u\<^esub> t"} if the states @{text s} and @{text t} are equivalent for the
+domain @{text u} in our view partitioning.\<close>
+
 abbreviation view' :: "'state \<Rightarrow> 'dom \<Rightarrow> 'state \<Rightarrow> bool" ("_ \<sim>\<^bsub>_\<^esub> _")
 where "(s \<sim>\<^bsub>u\<^esub> t) \<equiv> (s, t) \<in> view u"
+
+text \<open>Equivalence relations are reflexive, symmetric and transitive.\<close>
 
 lemma view_refl: "s \<sim>\<^bsub>u\<^esub> s"
   and view_sym: "(s \<sim>\<^bsub>u\<^esub> s') \<Longrightarrow> (s' \<sim>\<^bsub>u\<^esub> s)"
@@ -56,11 +87,24 @@ using view_equiv
 unfolding equiv_def refl_on_def sym_def trans_def
 by blast+
 
+text \<open>The unwinding theorem states that an automaton is secure wrt.\ a noninterference policy
+if the following three properties are satisfied for the given view partitioning.\<close>
+
+text \<open>@{emph \<open>Output consistency\<close>} requires that two states give the same output for an action
+@{text a}, if they are equivalent for the domain of that action. In other words, observers in
+a given domain cannot distinguish equivalent states via the outputs of their actions.\<close>
+
 definition "output_consistent
 \<equiv> \<forall>a s t. (s \<sim>\<^bsub>dom a\<^esub> t) \<longrightarrow> out s a = out t a"
 
+text \<open>@{emph \<open>Step consistency\<close>} requires that performing a visible action from two equivalent
+states again results in equivalent states.\<close>
+
 definition "step_consistent
 \<equiv> \<forall>s t u a. (((dom a) \<leadsto> u) \<and> (s \<sim>\<^bsub>u\<^esub> t)) \<longrightarrow> ((step s a) \<sim>\<^bsub>u\<^esub> (step t a))"
+
+text \<open>@{emph \<open>Local respect of @{text \<leadsto>}\<close>} requires that performing a secret action preserves the
+equivalence class of the current state.\<close>
 
 definition "locally_respects_FP
 \<equiv> \<forall>s u a. \<not>((dom a) \<leadsto> u) \<longrightarrow> (s \<sim>\<^bsub>u\<^esub> (step s a))"
@@ -73,17 +117,17 @@ The induction schema for lists looks as follows:
 
 We prove noninterference using a helper lemma: Instead of letting the lists of actions (unpurged
 and purged) run from the starting state, we let them run from two equivalent, but otherwise
-arbitrary states @{text s} and @{text t}, respectively. This makes the induction hypothesis much
-more useful, as we will see. Moreover, we focus first on showing that the states after the two runs
-are equivalent for an @{text l}-observer (when purging for @{text l}).
+arbitrary states @{text s} and @{text t}, respectively. This makes the induction hypothesis more
+useful. Moreover, we focus first on showing that the states after the two runs are equivalent for
+an observer in the domain @{text u} (when purging for @{text u}).
 \<close>
 
 lemma unwinding_lemma:
   assumes lr: "locally_respects_FP"
       and sc: "step_consistent"
-      and s_equiv_t: "s \<sim>\<^bsub>u\<^esub> t"
+      and "s \<sim>\<^bsub>u\<^esub> t"
   shows "(run s \<alpha>) \<sim>\<^bsub>u\<^esub> (run t (purge \<alpha> u))"
-using s_equiv_t
+using `s \<sim>\<^bsub>u\<^esub> t`
 proof (induction \<alpha> arbitrary: s t)
   case Nil
     -- \<open>Base case: empty list []\<close>
@@ -93,13 +137,14 @@ proof (induction \<alpha> arbitrary: s t)
     with `s \<sim>\<^bsub>u\<^esub> t` show "(run s []) \<sim>\<^bsub>u\<^esub> (run t (purge [] u))" by simp
 next
   case (Cons a' \<alpha>')
-    -- \<open>Induction step:\<close>
+    -- \<open>Inductive step:\<close>
     -- \<open>List starts with action @{text a'} and continues with list @{text \<alpha>'} (possibly empty).\<close>
     -- \<open>The following induction hypothesis about @{text \<alpha>'} is available
         (for any @{text s'} and @{text t'}):\<close>
     -- \<open>@{thm Cons.IH[of "s'" "t'"]}\<close>
+    -- \<open>We proceed by a case distinction whether @{text a'} is visible for @{text u} or not.\<close>
     show "(run s (a' # \<alpha>')) \<sim>\<^bsub>u\<^esub> (run t (purge (a' # \<alpha>') u))"
-    proof (cases "(dom a') \<leadsto> u")
+    proof (cases)
       assume flow: "(dom a') \<leadsto> u"
       with `s \<sim>\<^bsub>u\<^esub> t` have "(step s a') \<sim>\<^bsub>u\<^esub> (step t a')"
         using sc              -- \<open>Step consistency\<close>
@@ -125,7 +170,7 @@ next
     qed
 qed
 
-text \<open>With this lemma, noninterference directly follows by setting @{text "s = t = s0"} and
+text \<open>With this lemma, noninterference follows directly by setting @{text "s = t = s0"} and
 using output consistency.\<close>
 
 theorem unwinding_theorem:
@@ -133,7 +178,7 @@ theorem unwinding_theorem:
       and "locally_respects_FP"
       and "step_consistent"
   shows "NI_secure"
-using assms unwinding_lemma[where s = s0 and t = s0] view_refl
+using assms unwinding_lemma[where s = s0 and t = s0] view_refl[of s0]
 unfolding NI_secure_def output_consistent_def
 by auto
 
